cfg-list/aProdsScript.sml
@@ -13,8 +13,6 @@ val _ = new_theory "aProds";
 val _ = Globals.linewidth := 60
 val _ = set_trace "Unicode" 1
 
-fun MAGIC (asl, w) = ACCEPT_TAC (mk_thm(asl,w)) (asl,w);
-
 (* Greibach Normal Form *)
 
 (*
