cfg-list/cnfScript.sml
@@ -12,7 +12,6 @@ val _ = new_theory "cnf";
 val _ = Globals.linewidth := 60
 val _ = set_trace "Unicode" 1
 
-fun MAGIC (asl, w) = ACCEPT_TAC (mk_thm(asl,w)) (asl,w);
 
 val noeProds = Define
 `noeProds ru = ¬∃l. rule l [] ∈ ru`;
