cfg-list/unitProdsScript.sml
@@ -9,7 +9,6 @@ val _ = new_theory "unitProds"
 val _ = Globals.linewidth := 60
 val _ = set_trace "Unicode" 1
 
-fun MAGIC (asl, w) = ACCEPT_TAC (mk_thm(asl,w)) (asl,w);
 
 (* Rules of the form A->B, where A and B are in nonTerminals g *)
 val unitProds = Define 
