lib/treeDerivScript.sml
@@ -1,0 +1,179 @@
+(* A theory about parse trees *)
+open HolKernel boolLib bossLib Parse Defn BasicProvers
+
+open stringTheory grammarDefTheory symbolDefTheory listTheory pairTheory
+    optionTheory relationTheory boolSimps rich_listTheory pred_setTheory
+
+open listLemmasTheory parseTreeTheory grammarDefTheory relationLemmasTheory    
+
+val _ = new_theory "treeDeriv";
+
+val _ = Globals.linewidth := 60
+val _ = set_trace "Unicode" 1
+
+
+(* used to be lem1 in slr-parsing *)
+val treeRtc = store_thm("treeRtc",
+``(∀t. MEM t ptl ∧ isNode t ⇒ RTC (derives g) [ptree2Sym t] (MAP TS (leaves t))) 
+⇒  RTC (derives g) (MAP ptree2Sym ptl) (MAP TS (cleaves ptl))``,
+
+Induct_on `ptl` THEN  SRW_TAC [] [ptree2Sym_def, leaves_def, RTC_RULES] THEN
+Cases_on `h` THEN SRW_TAC [] [ptree2Sym_def, leaves_def] THEN
+FULL_SIMP_TAC (srw_ss() ++ DNF_ss) [isNode_def, ptree2Sym_def, leaves_def] 
+THENL[
+`RTC (derives g) [(TS t)] [(TS t)]` by METIS_TAC [RTC_RULES] THEN
+METIS_TAC [derives_append, APPEND],
+METIS_TAC [derives_append, APPEND]]);
+
+val vpt_rtcd = store_thm ("vpt_rtcd",
+``∀g t.validptree g t ⇒ 
+RTC (derives g) [ptree2Sym t] (MAP TS (leaves t))``,
+HO_MATCH_MP_TAC validptree_ind THEN SRW_TAC [] [] THEN
+FULL_SIMP_TAC (srw_ss()) [validptree] THEN
+`derives g [NTS n] (MAP ptree2Sym ptl)` by METIS_TAC [res1, getSymsEqptree2Sym] THEN
+Q_TAC SUFF_TAC `RTC (derives g) (MAP ptree2Sym ptl) (MAP TS (leaves (Node n ptl)))` 
+THENL[
+SRW_TAC [] [ptree2Sym_def] THEN METIS_TAC [RTC_RULES, getSymsEqptree2Sym],
+METIS_TAC [treeRtc, leaves_def]]);
+
+
+val leafRtcd = store_thm
+("leafRtcd",
+``∀t.isLeaf t ⇒ (derives g)^* [root t] (MAP TS (fringe t))``,
+
+Cases_on `t` THEN
+SRW_TAC [][isLeaf_def, root_def, fringe_def]);
+
+val ptlRtcd = store_thm
+("ptlRtcd",
+``∀ptl.(∀e.MEM e ptl ⇒ (derives g)^* [root e] (MAP TS (fringe e))) 
+ ⇒
+(derives g)^* (MAP root ptl) (MAP TS (FLAT  (MAP fringe ptl)))``,
+
+Induct_on `ptl` THEN SRW_TAC [][] THEN
+Cases_on `h` THEN FULL_SIMP_TAC (srw_ss()) [root_def, fringe_def] THEN1
+METIS_TAC [rtc_derives_same_append_left, APPEND] THEN
+`(derives g)^* [NTS n] (MAP TS (fringe (Node n l)))` by METIS_TAC [root_def] THEN
+FULL_SIMP_TAC (srw_ss()++boolSimps.ETA_ss) [fringe_def] THEN
+METIS_TAC [derives_append, APPEND]);
+
+
+val vptRtcd = store_thm
+("vptRtcd",
+``∀g t.validptree g t ⇒ (derives g)^* [root t] (MAP TS (fringe t))``,
+
+HO_MATCH_MP_TAC validptree_ind THEN
+SRW_TAC [][] THEN
+FULL_SIMP_TAC (srw_ss()) [root_def, validptree] THEN
+ `(∀e.MEM e ptl ⇒ (derives g)^* [root e] (MAP TS (fringe e)))` 
+ by (SRW_TAC [][] THEN
+     Cases_on `e` THEN 
+     FULL_SIMP_TAC (srw_ss()++boolSimps.ETA_ss) [root_def, fringe_def] THEN
+     FULL_SIMP_TAC (srw_ss()) [validptree] THEN
+     `isNode (Node n' l)` by SRW_TAC [][isNode_def] THEN
+     RES_TAC THEN
+     FULL_SIMP_TAC (srw_ss()++boolSimps.ETA_ss) [root_def, fringe_def]) THEN
+FULL_SIMP_TAC (srw_ss()) [validptree] THEN
+`(derives g)^* [NTS n] (MAP TS (FLAT (MAP fringe ptl)))` 
+by METIS_TAC [getSymsEqRoot, ptlRtcd, res1, RTC_RULES] THEN
+Cases_on `ptl=[]` THEN 
+FULL_SIMP_TAC (srw_ss()++boolSimps.ETA_ss) [getSymbols_def, fringe_def]);
+
+
+val lpexImpvpt = store_thm
+("lpexImpvpt",
+``∀l.(∀a b.MEM (a,b) l ⇒  
+   (isNonTmnlSym a ⇒ 
+    ∃t.validptree g t ∧ (MAP TS (fringe t) = b) ∧ (root t = a)) ∧
+      (isTmnlSym a ⇒ ([a]=b))) ⇒
+∃ts.(MAP root ts = MAP FST l) ∧ 
+(MAP TS (FLAT (MAP fringe ts)) = FLAT (MAP SND l)) ∧
+(∀e.MEM e ts ∧ isNode e ⇒ validptree g e)``,
+
+Induct_on `l` THEN SRW_TAC [][] THEN
+Cases_on `h` THEN
+Cases_on `q` THEN FULL_SIMP_TAC (srw_ss()) [] THEN1
+(`∃t.validptree g t ∧ (MAP TS (fringe t) = r) ∧ (root t = NTS n)`
+by METIS_TAC [isNonTmnlSym_def, symbol_11] THEN
+Q.EXISTS_TAC `t::ts` THEN
+SRW_TAC [][] THEN
+FULL_SIMP_TAC (srw_ss()) []) THEN
+Q.EXISTS_TAC `Leaf t::ts` THEN
+SRW_TAC [][root_def,fringe_def] THEN
+`[TS t]=r` by METIS_TAC [isTmnlSym_def] THEN
+METIS_TAC [APPEND, isNode_def]);
+
+
+val rtcdImpVpt = store_thm
+("rtcdImpVpt",
+``∀A y.(derives g) ⊢ dl ◁ [NTS A] → y ⇒ 
+ EVERY isTmnlSym y ⇒
+ ∃t.validptree g t ∧ (MAP TS (fringe t) = y) ∧ (root t = NTS A)``,
+
+completeInduct_on `LENGTH dl` THEN
+SRW_TAC [][] THEN
+Cases_on `dl` THEN1 
+FULL_SIMP_TAC (srw_ss()) [listderiv_def] THEN
+Cases_on `t` THEN FULL_SIMP_TAC (srw_ss()) [] THEN1
+
+(FULL_SIMP_TAC (srw_ss()) [derives_def, listderiv_def, lreseq] THEN
+ SRW_TAC [][] THEN
+ FULL_SIMP_TAC (srw_ss()) [isTmnlSym_def]) THEN
+
+`derives g h h' ∧ derives g ⊢ h'::t' ◁ h' → y` by METIS_TAC [listDerivHdBrk] THEN
+`h = [NTS A]` by FULL_SIMP_TAC (srw_ss()) [listderiv_def] THEN
+SRW_TAC [][] THEN
+`∃l.(h' = MAP FST l) ∧ (y = FLAT (MAP SND l)) ∧
+ ∀a b. MEM (a,b) l ⇒  ∃dl'. LENGTH dl' ≤ LENGTH (h'::t') ∧ 
+ derives g ⊢ dl' ◁ [a] → b` by METIS_TAC [listPairExistsLd] THEN
+SRW_TAC [][] THEN
+`∀a b.MEM (a,b) l ⇒
+ (isNonTmnlSym a ⇒ ∃t.validptree g t ∧ (MAP TS (fringe t) = b) ∧ 
+ (root t = a)) ∧ (isTmnlSym a ⇒ ([a]=b))` by
+(SRW_TAC [][] THEN
+RES_TAC THEN
+FULL_SIMP_TAC (srw_ss()) [] THEN
+`LENGTH dl' < SUC (SUC (LENGTH t'))` by DECIDE_TAC THEN
+FIRST_X_ASSUM (Q.SPECL_THEN [`LENGTH dl'`] MP_TAC) THEN SRW_TAC [][] THEN
+FIRST_X_ASSUM (Q.SPECL_THEN [`dl'`] MP_TAC) THEN SRW_TAC [][] THEN1
+(Cases_on `a` THEN FULL_SIMP_TAC (srw_ss()) [isNonTmnlSym_def] THEN
+FIRST_X_ASSUM (Q.SPECL_THEN [`n`,`b`] MP_TAC) THEN SRW_TAC [][] THEN
+`EVERY isTmnlSym b` by 
+ (FULL_SIMP_TAC (srw_ss()) [rgr_r9eq] THEN
+ SRW_TAC [][] THEN
+ FULL_SIMP_TAC (srw_ss()) [FLAT_APPEND]) THEN
+METIS_TAC []) THEN 
+Cases_on `a` THEN FULL_SIMP_TAC (srw_ss()) [isTmnlSym_def] THEN
+Cases_on `dl'` THEN FULL_SIMP_TAC (srw_ss()) [listderiv_def] THEN
+SRW_TAC [][] THEN
+Cases_on `t''` THEN FULL_SIMP_TAC (srw_ss()) [] THEN
+FULL_SIMP_TAC (srw_ss()) [derives_def, lreseq]) THEN
+`∃ts.(MAP root ts = MAP FST l) ∧ (MAP TS (FLAT (MAP fringe ts)) = FLAT (MAP SND l)) ∧
+(∀e.MEM e ts ∧ isNode e ⇒ validptree g e)`
+by METIS_TAC [lpexImpvpt] THEN
+FULL_SIMP_TAC (srw_ss()) [derives_def, lreseq] THEN
+Q.EXISTS_TAC `Node A ts` THEN
+SRW_TAC [boolSimps.ETA_ss][validptree, fringe_def, root_def] THEN
+METIS_TAC [getSymsEqRoot]);
+
+
+val ptLangThm = store_thm
+("ptLangThm",
+``∀w.w ∈ language g = 
+ ∃t.validptree g t ∧ (MAP TS (fringe t) = w) ∧
+ (root t = NTS (startSym g))``,
+
+SRW_TAC [][language_def, EXTENSION, EQ_IMP_THM] THEN
+FULL_SIMP_TAC (srw_ss()) [] THENL[
+
+IMP_RES_TAC rtc2list_exists' THEN
+METIS_TAC [rtcdImpVpt],
+
+METIS_TAC [vptRtcd, root_def],
+
+SRW_TAC [][EVERY_MEM] THEN
+Cases_on `e` THEN 
+FULL_SIMP_TAC (srw_ss()) [MEM_MAP, isTmnlSym_def]]);
+
+
+val _ = export_theory();
