pda/pumpingLemmaTreeScript.sml
@@ -1,0 +1,646 @@
+open HolKernel boolLib bossLib Parse BasicProvers Defn
+
+open pred_setTheory stringTheory containerTheory relationTheory
+listTheory rich_listTheory optionTheory arithmeticTheory
+
+
+open listLemmasTheory relationLemmasTheory grammarDefTheory
+     arithmeticLemmasTheory symbolDefTheory cnfTheory parseTreeTheory
+     treeDerivTheory
+
+val _ = new_theory "pumpingLemmaTree";
+
+fun MAGIC (asl, w) = ACCEPT_TAC (mk_thm(asl,w)) (asl,w);
+
+val _ = Globals.linewidth := 60
+val _ = set_trace "Unicode" 1
+
+
+val treeSyms_defn = Hol_defn "treeSyms_defn"
+`(treeSyms (Leaf tm) =  ([TS tm]:(α,β) symbol list)) ∧
+(treeSyms (Node n t) =  (NTS n) :: (FLAT (MAP treeSyms t)))`;
+
+val (treeSyms, treeSyms_ind) = tprove (treeSyms_defn,
+WF_REL_TAC (`measure ptsize`) THEN
+SRW_TAC [] [] THEN
+FULL_SIMP_TAC (srw_ss()) [rgr_r9eq, ptsizel_append] THEN
+DECIDE_TAC);
+
+val distinctSyms = Define
+`distinctSyms t = rmDupes (treeSyms t)`;
+
+val subtree = Define
+`(subtree t [] = SOME t) ∧
+(subtree (Node n ptl) (p::ps) = 
+ if (p < LENGTH ptl) then
+     subtree (EL p ptl) ps else NONE)`;
+
+val isSubtree = Define
+`isSubtree st t = ∃p. p ≠ [] ∧ (subtree t p = SOME st)`;
+
+val allTms = Define
+`allTms ptl = isWord (MAP ptree2Sym ptl)`;
+
+val btree = Define
+`btree B st t = (ptree2Sym st = NTS B) ∧  isSubtree st t`;
+
+val symRepProp = Define
+`symRepProp t0 t1 t =
+∃B. btree B t1 t ∧ btree B t0 t1`;
+
+val lastExpProp = Define
+`lastExpProp t = ∃t0 t1. symRepProp t0 t1 t ∧ 
+∃B n1 n2.(t1 = Node B y1 y2) ∧ (root y1 = n1) ∧ (root y2 = n2) ∧
+(¬∃st0 st1. symRepProp st0 st1 y1) ∧ (¬∃st0 st1. symRepProp st0 st1 y2)`;
+
+
+val max = Define
+`(max n [] = n) ∧
+(max n (x::xs) = if (n > x) then max n xs else max x xs)`;
+
+val height_defn = Hol_defn "height_defn"
+`(height (Leaf tm) = 0) ∧
+ (height (Node n l) = 1 + max 0 (MAP height l))`;
+
+
+val (height_def, height_ind) = tprove (height_defn,
+WF_REL_TAC (`measure ptsize`) THEN
+SRW_TAC [] [] THEN
+FULL_SIMP_TAC (srw_ss()) [rgr_r9eq, ptsizel_append] THEN
+DECIDE_TAC);
+
+
+val subtreeApp = store_thm
+("subtreeApp",
+``∀t t1 p p'.
+ (subtree t p = SOME t1) ∧ (subtree t1 p' = SOME t0) ⇒
+ (subtree t (p++p') = SOME t0)``,
+
+Induct_on `p` THEN SRW_TAC [][] THEN1
+(Cases_on `t` THEN FULL_SIMP_TAC (srw_ss()) [subtree]) THEN
+
+Cases_on `t` THEN
+FULL_SIMP_TAC (srw_ss()) [subtree] THEN
+Cases_on `h < LENGTH l` THEN FULL_SIMP_TAC (srw_ss()) []);
+
+
+val subtreeTrans = store_thm 
+("subtreeTrans",
+``∀t0 t1 t. isSubtree t1 t ∧ isSubtree t0 t1 ⇒ isSubtree t0 t``,
+
+FULL_SIMP_TAC (srw_ss()) [isSubtree] THEN
+SRW_TAC [][] THEN
+Q.EXISTS_TAC `p ++ p'` THEN
+SRW_TAC [][] THEN
+METIS_TAC [subtreeApp]);
+
+val subtImpisSubt = store_thm
+("subtImpisSubt",
+``∀t p t1. (subtree t p = SOME t1) ∧ p ≠ [] ⇒ isSubtree t1 t``,
+
+Induct_on `p` THEN SRW_TAC [][subtree] THEN
+Cases_on `t` THEN FULL_SIMP_TAC (srw_ss()) [subtree, isSubtree] THEN
+Cases_on `h < LENGTH l` THEN FULL_SIMP_TAC (srw_ss())[] THEN
+Cases_on `p` THEN FULL_SIMP_TAC (srw_ss()) [subtree] THEN1
+(Cases_on `EL h l` THEN FULL_SIMP_TAC (srw_ss()) [subtree] THEN
+ SRW_TAC [][] THEN
+ Q.EXISTS_TAC `[h]` THEN
+ SRW_TAC [][subtree]) THEN
+
+FIRST_X_ASSUM (Q.SPECL_THEN [`EL h l`, `t1`] MP_TAC) THEN SRW_TAC [][] THEN
+Q.EXISTS_TAC `h::h'::t` THEN
+SRW_TAC [][subtree]);
+
+
+val subtreeNotSymProp = store_thm
+("subtreeNotSymProp",
+``(subtree t p = SOME t1) ∧ p ≠ [] ∧ (¬∃s0 s1. symRepProp s0 s1 t) ⇒
+ ¬∃s0 s1. symRepProp s0 s1 t1``,
+
+SRW_TAC [][symRepProp] THEN
+SPOSE_NOT_THEN ASSUME_TAC THEN 
+FULL_SIMP_TAC (srw_ss()) [btree] THEN
+`isSubtree t1 t` by METIS_TAC [isSubtree] THEN
+METIS_TAC [subtreeTrans]);
+
+
+val subtreeLastExp = store_thm
+("subtreeLastExp",
+``∀t t1. lastExpProp t1 ∧ isSubtree t1 t ⇒
+ lastExpProp t``,
+
+SRW_TAC [][isSubtree, lastExpProp] THEN
+FULL_SIMP_TAC (srw_ss()) [symRepProp, btree] THEN
+Q.EXISTS_TAC `t0` THEN
+Q.EXISTS_TAC `t1'` THEN
+SRW_TAC [][] THEN1
+METIS_TAC [subtreeTrans, isSubtree]);
+
+val maxMapElem = store_thm
+("maxMapElem",
+``∀l n. (max n (MAP f l) = n') ⇒ 
+(∃e. MEM e l ∧ (f e = n')) ∨ (n = n')``,
+
+Induct_on `l` THEN SRW_TAC [][max] THEN
+FULL_SIMP_TAC (srw_ss()) [max] THEN
+METIS_TAC []);
+
+val subtreeHeight = store_thm
+("subtreeHeight",
+``∀t p t1. (subtree t p = SOME t1) ∧ p ≠ [] ⇒ height t1 < height t``,
+
+Induct_on `height t` THEN SRW_TAC [][] THEN1
+(Cases_on `t` THEN FULL_SIMP_TAC (srw_ss()) [height_def] THEN
+Cases_on `p` THEN FULL_SIMP_TAC (srw_ss()) [subtree]) THEN
+Cases_on `t` THEN FULL_SIMP_TAC (srw_ss()) [height_def] THEN
+`v = max 0 (MAP (λa. height a) l)` by DECIDE_TAC THEN
+SRW_TAC [][] THEN
+MAGIC);
+
+
+val symPropImpLastExp = store_thm
+("symPropImpLastExp",
+``∀t t0 t1. symRepProp t0 t1 t ⇒ lastExpProp t``,
+
+completeInduct_on `height t` THEN
+SRW_TAC [][] THEN
+Cases_on `t` THEN1
+(FULL_SIMP_TAC (srw_ss()) [lastExpProp, symRepProp, btree, isSubtree] THEN
+ Cases_on `p` THEN FULL_SIMP_TAC (srw_ss()) [subtree]) THEN
+
+FULL_SIMP_TAC (srw_ss()) [symRepProp] THEN
+`(ptree2Sym t1 = NTS B) ∧ isSubtree t1 (Node n l)` by METIS_TAC [btree] THEN
+`height t1 < height (Node n l)` by METIS_TAC [subtreeHeight, isSubtree] THEN
+Cases_on `∃s0 s1.symRepProp s0 s1 t1` THEN1
+
+(FULL_SIMP_TAC (srw_ss()) [symRepProp] THEN
+`lastExpProp t1` by METIS_TAC [] THEN
+METIS_TAC [subtreeLastExp]) THEN
+
+FULL_SIMP_TAC (srw_ss()) [symRepProp] THEN
+SRW_TAC [][lastExpProp] THEN
+Q.EXISTS_TAC `t0` THEN
+Q.EXISTS_TAC `t1` THEN
+SRW_TAC [][] THEN1
+(FULL_SIMP_TAC (srw_ss()) [symRepProp] THEN
+ METIS_TAC []) THEN
+
+FULL_SIMP_TAC (srw_ss()) [symRepProp] THEN
+SPOSE_NOT_THEN ASSUME_TAC THEN
+FULL_SIMP_TAC (srw_ss()) [btree] THEN
+METIS_TAC [subtreeTrans]);
+
+
+
+val cnfTree = store_thm
+("cnfTree",
+``∀g tree. validptree g tree ⇒ isCnf g ⇒ ∀n t. (tree = Node n t) ⇒
+    ∃n1 t1 n2 t2.(t = [Node n1 t1; Node n2 t2]) ∨ ∃ts.(t = [Leaf ts])``,
+
+HO_MATCH_MP_TAC validptree_ind THEN SRW_TAC [][] THEN
+FULL_SIMP_TAC (srw_ss()) [validptree, isCnf_def] THEN
+RES_TAC THEN
+FULL_SIMP_TAC (srw_ss()) [list_lem2, list_lem1] THEN1
+(Cases_on `e1` THEN Cases_on `e2` THEN
+ SRW_TAC [][] THEN
+ FULL_SIMP_TAC (srw_ss()) [isNonTmnlSym_def, isNode_def] THEN
+ MAGIC) THEN
+MAGIC);
+
+
+
+val inpLen = store_thm
+("inpLen",
+``∀g t. validptree g t ⇒
+ isCnf g  ⇒ 
+ (¬∃t0 t1. symRepProp t0 t1 t) ⇒
+ ∀k. (k = LENGTH (distinctSyms t)) ⇒
+ (LENGTH (leaves t) ≤ 2**(k - 1))``,
+
+HO_MATCH_MP_TAC validptree_ind THEN
+SRW_TAC [][] THEN
+IMP_RES_TAC cnfTree THEN
+FULL_SIMP_TAC (srw_ss()) [] THEN
+SRW_TAC [][] THEN
+FULL_SIMP_TAC (srw_ss()) [] THEN
+MAGIC);
+
+
+val inpLeninv = store_thm
+("inpLeninv",
+ ``isCnf g ∧ validptree g t ∧
+ LENGTH (leaves t) > 2**(k - 1) ∧
+ (k = LENGTH (distinctSyms t))
+  ⇒
+  ∃t0 t1. symRepProp t0 t1 t``,
+
+ SRW_TAC [][] THEN
+Q.ABBREV_TAC `k = LENGTH (distinctSyms t)` THEN
+`¬(LENGTH (leaves t) ≤ 2 ** (k − 1))` by DECIDE_TAC THEN
+METIS_TAC [inpLen]);
+
+
+
+val subtreeLevel = store_thm
+("subtreeLevel",
+``∀t p. (subtree t p = SOME t1) ∧ p ≠ [] ⇒
+   ∃n ptl. (subtree t (FRONT p) = SOME (Node n ptl)) ∧ MEM t1 ptl``,
+
+Induct_on `p` THEN SRW_TAC [][] THEN
+Cases_on `t` THEN FULL_SIMP_TAC (srw_ss()) [subtree] THEN
+Cases_on `h < LENGTH l` THEN FULL_SIMP_TAC (srw_ss()) [] THEN
+Cases_on `p` THEN FULL_SIMP_TAC (srw_ss()) [] THEN1
+
+(Cases_on `EL h l` THEN
+FULL_SIMP_TAC (srw_ss()) [subtree] THEN
+SRW_TAC [][] THEN
+METIS_TAC [EL_IS_EL]) THEN
+SRW_TAC [][subtree]);
+
+
+val numd = store_thm
+("numd",
+``∀t.LENGTH (distinctSyms t) ≥ 1``,
+
+Cases_on `t` THEN SRW_TAC [][distinctSyms, treeSyms, rmDupes, delete_def,
+			     rmDupes] THEN
+DECIDE_TAC);
+
+val numdLeqNtms = store_thm
+("numdLeqNtms",
+``∀g t. validptre g t ⇒ LENGTH (distinctSyms t) ≤ LENGTH (ntms g)``,
+
+HO_MATCH_MP_TAC validptree_ind THEN
+SRW_TAC [][] THEN
+FULL_SIMP_TAC (srw_ss()) [validptree, distinctSyms, treeSyms, rmDupes] THEN
+MAGIC);
+
+
+val vptTreeLevel = store_thm
+("vptTreeLevel",
+``∀g t.validptree g t ⇒ 
+∀t p t1. (subtree t p = SOME t1) ⇒
+∃pfx sfx. (fringe t = fringe pfx ++ fringe t1 ++ fringe sfx) ∧
+RTC (derives g) [root t] 
+(MAP TS (fringe pfx) ++ getSymbols [t1] ++ MAP TS (fringe sfx))``,
+
+
+HO_MATCH_MP_TAC validptree_ind THEN SRW_TAC [][] THEN
+FULL_SIMP_TAC (srw_ss()) [validptree] THEN
+MAGIC);
+
+
+val pumpCfg = store_thm
+("pumpCfg",
+``∀g.
+   isCnf (g:('a,'b) grammar)  ⇒
+   ∃n. n > 0 ∧
+       ∀z. z ∈ language g ∧ LENGTH z ≥ n ⇒
+           ∃u v w x y.
+	     (z = u ++ v ++ w ++ x ++ y) ∧
+             LENGTH v + LENGTH x ≥ 1 ∧
+             LENGTH v + LENGTH w + LENGTH x ≤ n ∧
+             ∀i. u++FLAT (lpow v i)++w++FLAT (lpow x i)++y ∈ language g``,
+
+SRW_TAC [][] THEN
+ Q.ABBREV_TAC `k=LENGTH (ntms g)` THEN
+Q.EXISTS_TAC `2**k` THEN
+SRW_TAC [][] THEN1 SRW_TAC [][Abbr`k`, GREATER_DEF] THEN
+`∃t. validptree g t ∧ (ptree2Sym t = NTS (startSym g)) ∧ (z = leaves t)` 
+ by MAGIC THEN
+SRW_TAC [][] THEN
+Q.ABBREV_TAC `z:(α,β) symbol list = leaves t` THEN
+Q.ABBREV_TAC `k0 = LENGTH (distinctSyms t)` THEN
+`k0 ≥ 1` by METIS_TAC [numd] THEN
+`k0 ≤ k` by METIS_TAC [numdLeqNtms] THEN
+`1 ≤ k0`by DECIDE_TAC THEN
+`k ≠ 0`by DECIDE_TAC THEN
+ `LENGTH z ≥ 2 ** k0` by METIS_TAC [powGtTrans] THEN
+ `LENGTH z > 2**(k0-1)` by METIS_TAC [powGt] THEN
+`∃t0 t1. symRepProp t0 t1 t` by METIS_TAC [inpLeninv] THEN
+IMP_RES_TAC symPropImpLastExp THEN
+`∃s0 s1. symRepProp s0 s1 t ∧ ¬∃st0 st1. symRepProp st0 st1 s0` 
+ by METIS_TAC [lastExpProp] THEN
+`∃B. btree B s1 t ∧ btree B s0 s1` by METIS_TAC [symRepProp] THEN
+FULL_SIMP_TAC (srw_ss()) [btree, isSubtree] THEN
+`∃n1 ptl1. (subtree t (FRONT p) = SOME (Node n1 ptl1)) ∧ s1 ∈ ptl1` 
+by METIS_TAC [subtreeLevel] THEN
+`RTC (derives g) [root t] (getSymbols ptl1)` by MAGIC THEN
+`∃pfx1 sfx1. (derives g)^* [root t] (getSymbols (pfx1++[s1]++sfx1)) ∧
+	     (ptl1 = pfx1 ++ [s1] ++ sfx1)` by METIS_TAC [rgr_r9eq] THEN
+SRW_TAC [][] THEN
+
+`∃n0 ptl0. (subtree s1 (FRONT p') = SOME (Node n0 ptl0)) ∧ s0 ∈ ptl0` 
+by METIS_TAC [subtreeLevel] THEN
+`RTC (derives g) [root s1] (getSymbols ptl0)` by MAGIC THEN
+`∃pfx0 sfx0. (derives g)^* [root s1] (getSymbols (pfx0++[s0]++sfx0)) ∧
+	     (ptl0 = pfx0 ++ [s0] ++ sfx0)` by METIS_TAC [rgr_r9eq] THEN
+SRW_TAC [][] THEN
+
+
+
+
+
+`validptree g s0` by MAGIC THEN
+`LENGTH (leaves s0) ≤ 2 ** (LENGTH (distinctSyms s0) - 1)`
+by METIS_TAC [inpLen] THEN
+
+
+FULL_SIMP_TAC (srw_ss()) [btree, isSubtree] THEN
+
+`∃n ptl. (subtree s1 (FRONT p') = SOME (Node n ptl)) ∧ s0 ∈ ptl` 
+by METIS_TAC [subtreeLevel] THEN
+
+`∃n1 ptl1. (subtree t (FRONT p) = SOME (Node n1 ptl1)) ∧ s1 ∈ ptl1` 
+by METIS_TAC [subtreeLevel] THEN
+
+
+
+
+∃v0 x0. s1 -> getSyms (v0 ++ s0 ++ x0)
+
+
+
+
+Cases_on `t` THEN
+FULL_SIMP_TAC (srw_ss()) [subtree]
+	     
+  ∃pfx sfx. RTC (derives g) [root t] (getSymbols (pfx ++ t1 ++ sfx))``
+
+
+ `symRepProp t` by MAGIC THEN
+FULL_SIMP_TAC (srw_ss()) [symRepProp] THEN
+SRW_TAC [][] THEN
+
+u = leaves pfx
+
+v = leaves pfx1
+
+w = leaves bst1
+
+x = leaves sfx1
+
+y = leaves sfx
+
+
+
+`z ∈ llanguage g` by METIS_TAC [drd_ld_langeq] THEN
+`(lderives g)^* [NTS (startSym g)] z ∧ EVERY isTmnlSym z`
+  by FULL_SIMP_TAC (srw_ss()) [llanguage_def] THEN
+`∃dl.(lderives g) ⊢ dl ◁ [NTS (startSym g)] → z`
+  by METIS_TAC [rtc2list_exists'] THEN
+Q.ABBREV_TAC `k0=LENGTH (distinctldNts dl)` THEN
+`LENGTH (distinctldNts dl) ≥ 1` by METIS_TAC [numdlds] THEN
+`k0 ≥ 1 ⇒ 1 ≤ k0` by DECIDE_TAC THEN
+`isNonTmnlSym (NTS (startSym g))` by METIS_TAC [isNonTmnlSym_def] THEN
+IMP_RES_TAC dldntsLeg THEN
+FULL_SIMP_TAC (srw_ss()) [isNonTmnlSym_def] THEN
+`MEM (startSym g) (ntms g)` by
+(SRW_TAC [][ntms_def, ntList_def, nonTerminalsList_def] THEN
+ METIS_TAC [rmd_r2, MEM, APPEND]) THEN
+`k0 ≤ k` by METIS_TAC [dldntsLeg] THEN
+ `1 ≤ k0` by METIS_TAC [] THEN
+`k ≠ 0` by DECIDE_TAC THEN
+ `LENGTH z ≥ 2 ** k0` by METIS_TAC [powGtTrans] THEN
+ `LENGTH z > 2**(k0-1)` by METIS_TAC [powGt] THEN
+ `symRepProp dl` by METIS_TAC [inpLeninv,symRepProp_def] THEN
+`EVERY isNonTmnlSym ([NTS (startSym g)]:('a,'b) symbol list)`
+by METIS_TAC [APPEND_ASSOC,APPEND_11,symbol_11,isNonTmnlSym_def,EVERY_DEF] THEN
+ `∃pz0:('a,'b) symbol list sz0:('a,'b) symbol list.([NTS (startSym g)]=pz0++sz0) ∧
+	 EVERY isTmnlSym pz0 ∧ EVERY isNonTmnlSym sz0`
+ by METIS_TAC [EVERY_DEF,APPEND_NIL] THEN
+`lastExpProp (g,dl,z)`
+by METIS_TAC [lastExp,symbol_11] THEN
+FULL_SIMP_TAC (srw_ss()) [lastExpProp] THEN
+SRW_TAC [][] THEN
+`lderives g ⊢ (dl1++TL dl2) ◁ [NTS n1]++[NTS n2] → (v++rst)` by
+METIS_TAC [listderivTrans, APPEND] THEN
+`∃pfx sfx.([NTS n1]++[NTS n2]=pfx++sfx) ∧ EVERY isTmnlSym pfx ∧
+	 EVERY isNonTmnlSym sfx` by
+(MAP_EVERY Q.EXISTS_TAC [`[]`,`[NTS n1]++[NTS n2]`] THEN
+ SRW_TAC [][isNonTmnlSym_def]) THEN
+`∃dl1' dl2' zb zy.
+   splitDerivProp (g,dl1++TL dl2,v++rst)
+   (dl1',[NTS n1],zb) (dl2',[NTS n2],zy)` by METIS_TAC [ldSplitDeriv,EVERY_APPEND] THEN
+FULL_SIMP_TAC (srw_ss()) [splitDerivProp] THEN
+SRW_TAC [][] THEN
+`LENGTH zb ≤ 2**(LENGTH (distinctldNts dl1') -1)`
+by METIS_TAC [symRepProp_def, inpLen,EVERY_APPEND] THEN
+`LENGTH zy ≤ 2**(LENGTH (distinctldNts dl2') -1)`
+by METIS_TAC [symRepProp_def, inpLen,EVERY_APPEND] THEN
+SRW_TAC [][] THEN
+`∃v''.zb++zy=v++v''`by
+(IMP_RES_TAC twoListAppEq THEN
+ FULL_SIMP_TAC (srw_ss()) [] THEN SRW_TAC [][] THEN
+ METIS_TAC [APPEND_ASSOC]) THEN
+SRW_TAC [][] THEN
+`lderives g ⊢ MAP (listsec v []) dl2 ◁
+   listsec v [] (v ++ ([NTS B]++w)) → listsec v [] (v ++ v'')`
+by METIS_TAC [listsecldSfxNil,APPEND_ASSOC,EVERY_APPEND] THEN
+FULL_SIMP_TAC (srw_ss()) [listsecDropNilSfx] THEN
+`¬symRepProp (MAP (listsec v []) dl2)` by METIS_TAC [notspropLsTmnls,
+						    APPEND_ASSOC,
+						    EVERY_APPEND] THEN
+`MEM (v++[NTS B]++w) dl1` by
+(Cases_on `dl1` THEN FULL_SIMP_TAC (srw_ss()) [listderiv_def] THEN
+ METIS_TAC [MEM, MEM_APPEND, APPEND_FRONT_LAST]) THEN
+`v ++ [NTS B] ++ w = v ++ ([NTS B]++w)` by SRW_TAC [][] THEN
+`∃p1 p2.([NTS B]++w = p1++p2) ∧ EVERY isTmnlSym p1 ∧ EVERY isNonTmnlSym p2`
+by METIS_TAC [ldMemlderivesSfx] THEN
+`∃dl1' dl2' zb' zy'.
+   splitDerivProp (g,(MAP (listsec v []) dl2),v'') (dl1',[NTS B],zb')
+   (dl2',w,zy')`
+by METIS_TAC [APPEND,ldSplitDeriv] THEN
+FULL_SIMP_TAC (srw_ss()) [splitDerivProp] THEN
+SRW_TAC [][] THEN
+FULL_SIMP_TAC (srw_ss()) [] THEN
+SRW_TAC [][] THEN
+MAP_EVERY Q.EXISTS_TAC [`tsl`,`v`,`zb'`,`zy'`,`rst'`] THEN
+SRW_TAC [][] THEN1
+(FULL_SIMP_TAC (srw_ss()) [ntProp] THEN SRW_TAC [][]
+ THENL[
+       `LENGTH ([NTS B;NTS n2]) > 1` by
+       FULL_SIMP_TAC (srw_ss()++ARITH_ss) [] THEN
+       `v ≠ [] ∨ w ≠ []` by METIS_TAC [cnfvwNotNil] THEN1
+       (`LENGTH v ≠ 0` by METIS_TAC [LENGTH_NIL] THEN DECIDE_TAC) THEN
+       `p1 = []` by (Cases_on `p1` THEN SRW_TAC [][] THEN
+		     Cases_on `h` THEN SRW_TAC [][] THEN
+		     FULL_SIMP_TAC (srw_ss()) [isTmnlSym_def,
+					       isNonTmnlSym_def]) THEN
+       SRW_TAC [][] THEN FULL_SIMP_TAC (srw_ss()) [] THEN
+       FULL_SIMP_TAC (srw_ss()) [] THEN
+       `zy' ≠ []` by METIS_TAC [cnfNotLderivesNilAllntms,
+				EVERY_DEF, APPEND_NIL] THEN
+       `LENGTH zy' ≠ 0` by METIS_TAC [LENGTH_NIL] THEN
+       DECIDE_TAC,
+
+       `LENGTH ([NTS n1;NTS n2]) > 1` by
+       FULL_SIMP_TAC (srw_ss()++ARITH_ss) [] THEN
+       `v ≠ [] ∨ w ≠ []` by METIS_TAC [cnfvwNotNil] THEN1
+       (`LENGTH v ≠ 0` by METIS_TAC [LENGTH_NIL] THEN DECIDE_TAC) THEN
+       `p1 = []` by (Cases_on `p1` THEN SRW_TAC [][] THEN
+		     Cases_on `h` THEN SRW_TAC [][] THEN
+		     FULL_SIMP_TAC (srw_ss()) [isTmnlSym_def,
+					       isNonTmnlSym_def]) THEN
+       SRW_TAC [][] THEN FULL_SIMP_TAC (srw_ss()) [] THEN
+       FULL_SIMP_TAC (srw_ss()) [] THEN
+       `zy' ≠ []` by METIS_TAC [cnfNotLderivesNilAllntms,
+				EVERY_DEF, APPEND_NIL] THEN
+       `LENGTH zy' ≠ 0` by METIS_TAC [LENGTH_NIL] THEN
+       DECIDE_TAC])
+THENL[
+      `LENGTH (distinctldNts dl1') ≤
+      LENGTH (distinctldNts (dl1 ++ TL dl2))` by METIS_TAC [distElemLen_def] THEN
+      `LENGTH (distinctldNts dl2') ≤
+      LENGTH (distinctldNts (dl1 ++ TL dl2))` by METIS_TAC [distElemLen_def] THEN
+      `LENGTH (zb ++ zy) = LENGTH (v ++ zb' ++ zy')`
+      by METIS_TAC [APPEND_ASSOC] THEN
+      FULL_SIMP_TAC (srw_ss()) [] THEN
+      `dl2 ≠ []` by (Cases_on `dl2` THEN
+		     FULL_SIMP_TAC (srw_ss()) [listderiv_def]) THEN
+      `∀e. (MEM e dl1 ⇒ MEM (tsl ++ e ++ sfx) dl)
+      ∧ (∀e. MEM e dl2 ⇒ MEM (tsl ++ e ++ sfx) dl) ⇒
+      LENGTH (distinctldNts (dl1++TL dl2)) ≤ LENGTH (distinctldNts dl)` by
+      METIS_TAC [dldntsLenLe, APPEND_NIL] THEN
+      `∀e. (MEM e dl1 ⇒ MEM (tsl ++ e ++ sfx) dl)
+      ∧ (∀e. MEM e dl2 ⇒ MEM (tsl ++ e ++ sfx) dl) ⇒
+      LENGTH (distinctldNts (dl1++TL dl2)) ≤ k` by
+      METIS_TAC [DECIDE ``a ≤ b ∧ b ≤ c ⇒ a ≤ c``] THEN
+      FULL_SIMP_TAC (srw_ss()) [distElemLen_def] THEN
+      `LENGTH (distinctldNts dl1') ≤ k`
+      by METIS_TAC [DECIDE ``a ≤ b ∧ b ≤ c ⇒ a ≤ c``] THEN
+      `LENGTH (distinctldNts dl2') ≤ k`
+      by METIS_TAC [DECIDE ``a ≤ b ∧ b ≤ c ⇒ a ≤ c``] THEN
+      `LENGTH zb ≤ 2 ** (k-1)` by METIS_TAC [powLe] THEN
+      `LENGTH zy ≤ 2 ** (k-1)` by METIS_TAC [powLe] THEN
+      `LENGTH zb + LENGTH zy ≤ 2**(k-1) + 2**(k-1)`by DECIDE_TAC THEN
+       `LENGTH zb + LENGTH zy ≤ 2*2**(k-1)`by DECIDE_TAC THEN
+       `LENGTH zb + LENGTH zy ≤ 2**(k-1+1)`by METIS_TAC [powMult] THEN
+       `LENGTH dl > 1` by
+       (SPOSE_NOT_THEN ASSUME_TAC THEN
+	Cases_on `dl` THEN FULL_SIMP_TAC (srw_ss()) [listderiv_def] THEN
+	Cases_on `t` THEN FULL_SIMP_TAC (srw_ss()++ARITH_ss) [] THEN
+	SRW_TAC [][] THEN
+	`EVERY isTmnlSym (pz0++sz0)` by METIS_TAC [EVERY_APPEND] THEN
+	Cases_on `pz0` THEN FULL_SIMP_TAC (srw_ss()) [] THEN
+	SRW_TAC [][] THEN
+	FULL_SIMP_TAC (srw_ss()) [isTmnlSym_def]) THEN
+       `k0 ≥ 1` by METIS_TAC [dldntsGe1] THEN
+       `k - 1 + 1 = k` by DECIDE_TAC THEN
+       METIS_TAC [],
+
+       FULL_SIMP_TAC (srw_ss()) [language_def,llanguage_def, EXTENSION] THEN
+       SRW_TAC [][]
+       THENL[
+	     (* 3 subgoals *)
+
+	     (* 1 *)
+	     FULL_SIMP_TAC (srw_ss()) [ntProp] THEN
+	     (Cases_on `p` THEN FULL_SIMP_TAC (srw_ss()) [] THEN1
+	      (`(tsl ++ [NTS B] ++ sfx) = pz0++sz0`
+	      by FULL_SIMP_TAC (srw_ss()) [listderiv_def] THEN
+	      `(tsl ++ [NTS B] ++ sfx = [NTS (startSym g)])`
+	      by METIS_TAC [] THEN
+	      FULL_SIMP_TAC (srw_ss()) [lreseq] THEN SRW_TAC [][] THEN
+
+	      `(lderives g)^* [NTS (startSym g)] (pfx++sfx')`
+	      by METIS_TAC [ldMemRel, APPEND, APPEND_NIL, APPEND_ASSOC] THEN
+
+	      `dl1 ≠ []` by (Cases_on `dl1` THEN FULL_SIMP_TAC (srw_ss()) [listderiv_def]) THEN
+	      `(lderives g)^* (pfx++sfx') (v ++ [NTS (startSym g)] ++ w)`
+	      by METIS_TAC [rtc2listRtcHdLast, listderiv_def, APPEND_ASSOC] THEN
+
+	      `dl1'' ≠ []` by (Cases_on `dl1''` THEN FULL_SIMP_TAC (srw_ss()) [listderiv_def]) THEN
+	      `(lderives g)^* [NTS (startSym g)] zb'`
+	      by METIS_TAC [rtc2listRtcHdLast, listderiv_def, APPEND_ASSOC] THEN
+
+	      `dl2'' ≠ []` by (Cases_on `dl2''` THEN FULL_SIMP_TAC (srw_ss()) [listderiv_def]) THEN
+	      `(lderives g)^* w zy'`
+	      by METIS_TAC [rtc2listRtcHdLast, listderiv_def, APPEND_ASSOC] THEN
+	      `(lderives g)^* [NTS (startSym g)] (v ++ [NTS (startSym g)] ++ w)`
+	      by METIS_TAC [RTC_RTC] THEN
+	      `(lderives g)^* v v` by SRW_TAC [][] THEN
+	      `(lderives g)^* [NTS (startSym g)]
+	     (FLAT (lpow v i) ++ zb' ++ FLAT (lpow zy' i))`
+	      by METIS_TAC [rtcDerivesReplEnd] THEN
+	      `rst' = []` by
+	      (Cases_on `dl3`  THEN FULL_SIMP_TAC (srw_ss()) [listderiv_def] THEN
+	       SRW_TAC [][] THEN
+	       Cases_on `t` THEN FULL_SIMP_TAC (srw_ss()) [lderives_def]) THEN
+	      SRW_TAC [][] THEN FULL_SIMP_TAC (srw_ss()) [] THEN
+	      `llanguage g = language g` by METIS_TAC [drd_ld_langeq] THEN
+	      FULL_SIMP_TAC (srw_ss()) [language_def, llanguage_def, EXTENSION] THEN
+	      METIS_TAC [EVERY_APPEND, islpowTmnl]) THEN
+
+	     `h = pz0++sz0` by FULL_SIMP_TAC (srw_ss()) [listderiv_def] THEN
+	     SRW_TAC [][] THEN
+
+	      `(lderives g)^* [NTS (startSym g)] (tsl ++ pfx++sfx'++sfx)`
+	      by METIS_TAC [ldMemRel, APPEND, APPEND_ASSOC] THEN
+
+	      `dl1 ≠ []` by (Cases_on `dl1` THEN FULL_SIMP_TAC (srw_ss()) [listderiv_def]) THEN
+	      `(lderives g)^* (pfx++sfx') (v ++ [NTS B] ++ w)`
+	      by METIS_TAC [rtc2listRtcHdLast, listderiv_def, APPEND_ASSOC] THEN
+
+	      `dl1'' ≠ []` by (Cases_on `dl1''` THEN FULL_SIMP_TAC (srw_ss()) [listderiv_def]) THEN
+	      `(lderives g)^* [NTS B] zb'`
+	      by METIS_TAC [rtc2listRtcHdLast, listderiv_def, APPEND_ASSOC] THEN
+
+
+	      `dl3 ≠ []` by (Cases_on `dl3` THEN FULL_SIMP_TAC (srw_ss()) [listderiv_def]) THEN
+	      `(lderives g)^* sfx rst'`
+	      by METIS_TAC [rtc2listRtcHdLast, listderiv_def, APPEND_ASSOC] THEN
+
+	      `dl2'' ≠ []` by (Cases_on `dl2''` THEN FULL_SIMP_TAC (srw_ss()) [listderiv_def]) THEN
+	      `(lderives g)^* w zy'`
+	      by METIS_TAC [rtc2listRtcHdLast, listderiv_def, APPEND_ASSOC] THEN
+	      `(lderives g)^* [NTS (startSym g)] (tsl ++ v ++ [NTS B] ++ w ++sfx)`
+	      by METIS_TAC [RTC_RTC, rtc_lderives_same_append_left,
+			    rtc_lderives_same_append_right, APPEND_ASSOC] THEN
+	      `(lderives g)^* [NTS B] (pfx++sfx')` by
+	      (`lderives g (tsl ++ [NTS B] ++ sfx)
+	       (tsl ++ pfx ++ sfx' ++ sfx)`
+	       by METIS_TAC [ldMemRel', APPEND, APPEND_ASSOC] THEN
+	       FULL_SIMP_TAC (srw_ss()) [lderives_def] THEN
+	       SRW_TAC [][] THEN
+	      `EVERY isNonTmnlSym [NTS lhs]` by SRW_TAC [][isNonTmnlSym_def] THEN
+	       `(s1=tsl) ∧ ([NTS lhs] ++ s2 = [NTS B]++sfx)`
+	       by METIS_TAC [symlistdiv3, NOT_CONS_NIL] THEN
+	       FULL_SIMP_TAC (srw_ss()) [] THEN
+	       SRW_TAC [][] THEN
+	       `rhs = pfx++sfx'` by METIS_TAC [APPEND_11, APPEND_ASSOC] THEN
+	       METIS_TAC [ldres1, RTC_RULES]) THEN
+	      `(lderives g)^* [NTS B] (v ++ [NTS B] ++ w)`
+	      by METIS_TAC [RTC_RTC] THEN
+	      `(lderives g)^* v v` by SRW_TAC [][] THEN
+	      `(lderives g)^* [NTS B]
+                 (FLAT (lpow v i) ++ zb' ++ FLAT (lpow zy' i))`
+	      by METIS_TAC [rtcDerivesReplEnd] THEN
+	      `llanguage g = language g` by METIS_TAC [drd_ld_langeq] THEN
+	      FULL_SIMP_TAC (srw_ss()) [language_def, llanguage_def, EXTENSION] THEN
+	      `(lderives g)^* (pz0++sz0) (tsl ++ [NTS B] ++sfx)`
+	      by METIS_TAC [ldMemRel, APPEND, APPEND_ASSOC] THEN
+	      `(lderives g)^* (pz0++sz0)
+		 (tsl ++ (FLAT (lpow v i) ++ zb' ++ FLAT (lpow zy' i)) ++ sfx)`
+	      by METIS_TAC [EVERY_APPEND, islpowTmnl, RTC_RTC,
+			    rtc_lderives_same_append_right,
+			    rtc_lderives_same_append_left] THEN
+	      `(lderives g)^*
+		 (tsl ++ FLAT (lpow v i) ++ zb' ++ FLAT (lpow zy' i) ++ sfx)
+		 (tsl ++ FLAT (lpow v i) ++ zb' ++ FLAT (lpow zy' i) ++ rst')`
+	      by METIS_TAC [APPEND_ASSOC, EVERY_APPEND, islpowTmnl,
+			    rtc_lderives_same_append_left] THEN
+	      `(lderives g)^* (pz0++sz0)
+		 (tsl ++ FLAT (lpow v i) ++ zb' ++ FLAT (lpow zy' i) ++ rst')`
+	      by METIS_TAC [RTC_RTC, APPEND_ASSOC] THEN
+	      METIS_TAC [EVERY_APPEND, islpowTmnl]),
+
+	      METIS_TAC [islpowTmnl],
+
+	      METIS_TAC [islpowTmnl]
+	      ]]
+
+
+MAGIC);
+
+val _ = export_theory ();
