slr-parsing/ambiguityScript.sml
@@ -10,8 +10,6 @@ yaccDefTheory parseProp1DefTheory parseProp2DefTheory
 lrGrammarDefTheory validItemInvTheory macStepTheory complDefTheory
 
 
-fun MAGIC (asl, w) = ACCEPT_TAC (mk_thm(asl,w)) (asl,w) 
-
 val _ = Globals.linewidth := 60
 
 val _ = set_trace "Unicode" 1
